More work in progress

src/Decide.v
@@ -15,222 +15,95 @@ Require Import Category.Theory.Functor.
 Require Import Solver.Lib.
 Require Import Solver.Expr.
 Require Import Solver.Denote.
-Require Import Solver.Normal.
 
 Generalizable All Variables.
 
 Section Decide.
 
-Open Scope partial_scope.
-
-Definition subst_all_expr (x : Expr) (xs : list (Expr * Expr)) : Expr := x.
-
-Program Fixpoint expr_forward
-        {C : Category}
-        (objs : obj_idx -> C)
-        (arrs : ∀ f : arr_idx, option (∃ x y, objs x ~{C}~> objs y))
-        (t : Expr)
-        (hyp : Expr)
-        (cont : forall C objs' arrs' defs',
-           [@expr_denote C objs' arrs' (subst_all_expr t defs')]) :
-  [expr_denote objs arrs hyp -> expr_denote objs arrs t] :=
-  match hyp with
-  | Top           => Reduce (cont C objs arrs nil)
-  | Bottom        => Yes
-  | Equiv x y f g => No         (* jww (2017-08-02): TODO *)
-  | Not p         => Reduce (cont C objs arrs nil)
-  | And p q       => No         (* jww (2017-08-02): TODO *)
-  | Or p q        => if expr_forward objs arrs t p cont
-                     then Reduce (expr_forward objs arrs t q cont)
-                     else No
-  | Impl _ _      => Reduce (cont C objs arrs nil)
-  end.
-Next Obligation. contradiction. Defined.
-Next Obligation. intuition. Defined.
-
-Program Fixpoint expr_backward
-        {C : Category}
-        (objs : obj_idx -> C)
-        (arrs : ∀ f : arr_idx, option (∃ x y, objs x ~{C}~> objs y))
-        (t : Expr)
-        {measure (expr_size t)} : [expr_denote objs arrs t] :=
-  match t with
-  | Top           => Yes
-  | Bottom        => No
-  | Equiv x y f g => match ArrowList_beq (normalize f) (normalize g) with
-                     | true  => Yes
-                     | false => No
-                     end
-  | Not p         => match expr_backward objs arrs p with
-                     | Proved _ _  => No
-                     | Uncertain _ => Yes
-                     end
-  | And p q       => match expr_backward objs arrs p with
-                     | Proved _ _  => Reduce (expr_backward objs arrs q)
-                     | Uncertain _ => No
-                     end
-  | Or p q        => match expr_backward objs arrs p with
-                     | Proved _ _  => Yes
-                     | Uncertain _ => Reduce (expr_backward objs arrs q)
-                     end
-  | Impl p q      => expr_forward objs arrs q p
-                       (fun C objs' arrs' defs' =>
-                          @expr_backward C objs' arrs' (subst_all_expr q defs') _)
-  end.
+Program Instance term_denote_proper C objs arrs dom cod :
+  Proper ((fun x y => term_beq x y = true) ==> @equiv _ (@option_setoid _ _))
+         (@term_denote C objs arrs dom cod).
 Next Obligation.
-  destruct f; simpl.
-  destruct (term_denote _ _ f) eqn:?;
-  destruct (term_denote _ _ g) eqn:?.
-  destruct (term_denote _ _ _).
-Admitted.
-Next Obligation.
-  induction p; simpl in *; auto.
-Admitted.
-Next Obligation.
-  abstract omega.
+  proper.
+  generalize dependent y;
+  generalize dependent cod;
+  generalize dependent dom;
+  induction x; simpl in *; intros.
+  - destruct y; repeat equalities; reflexivity.
+  - destruct y0; try discriminate.
+    repeat equalities.
+    destruct (arrs _); auto.
+    destruct s, s; equalities.
+    do 4 (equalities'; auto).
+    simpl_eq; reflexivity.
+  - destruct y; try discriminate.
+    repeat equalities.
+    specialize (IHx1 m0 cod _ H2).
+    specialize (IHx2 dom m0 _ H1).
+    destruct (term_denote _ _ _ _ x1) eqn:?;
+    destruct (term_denote _ _ _ _ y1) eqn:?;
+    try discriminate;
+    destruct (term_denote _ _ _ _ x2) eqn:?;
+    destruct (term_denote _ _ _ _ y2) eqn:?;
+    try discriminate; auto.
+    rewrite IHx1, IHx2; reflexivity.
 Defined.
 
-Theorem normalize_sound {p dom cod f} :
-  Term_well_typed arrs dom cod p ->
-  normalize_denote dom cod (normalize p) = Some f ->
-  ∃ f', f ≈ f' ∧ denote dom cod p = Some f'.
+Lemma term_denote_term_append C objs arrs x m y f1 f2 f' g' :
+  term_denote objs arrs m y (term_append f1 (Identity m)) ≈ Some f' ->
+  term_denote objs arrs x m (term_append f2 (Identity x)) ≈ Some g' ->
+  @term_denote C objs arrs x y (term_append (Compose m f1 f2) (Identity x)) ≈ Some (f' ∘ g').
 Proof.
-  generalize dependent cod.
-  generalize dependent dom.
-  induction p as [o|a|]; simpl in *; intros; equalities.
-  - exists f; repeat equalities; reflexivity.
-  - exists f.
-    destruct (get_arr a); [|discriminate].
-    repeat equalities; reflexivity.
-  - apply normalize_compose in H0; equalities; subst.
-    + destruct (Eq_eq_dec (ArrowList_dom arrs (normalize p1))
-                          (TermCod arrs p2)).
-      * rewrite <- e in *.
-        destruct (IHp1 _ _ _ H1 a2), (IHp2 _ _ _ H2 b0).
-        equalities.
-        rewrite e3, e1.
-        eexists; intuition.
-        now rewrite <- e0, <- e2.
-      * pose proof (ArrowList_normalize_dom_cod_sound arrs H2);
-        equalities.
-        now rewrite a1 in H3.
-    + clear IHp1 IHp2.
-      pose proof (ArrowList_normalize_dom_cod_sound arrs H1).
-      pose proof (ArrowList_normalize_dom_cod_sound arrs H2).
-      equalities.
-      now rewrite H3.
-Qed.
-
-Theorem normalize_sound_r {p dom cod f} :
-  Term_well_typed arrs dom cod p ->
-  denote dom cod p = Some f ->
-  ∃ f', f ≈ f' ∧ normalize_denote dom cod (normalize p) = Some f'.
-Proof.
-  generalize dependent cod.
-  generalize dependent dom.
-  induction p as [o|a|]; simpl in *; intros; equalities.
-  - exists f; repeat equalities; reflexivity.
-  - exists f.
-    destruct (get_arr a); [|discriminate].
-    repeat equalities; reflexivity.
-  - destruct (denote (TermCod arrs p2) cod p1) eqn:?; [|discriminate].
-    destruct (denote dom (TermCod arrs p2) p2) eqn:?; [|discriminate].
-    destruct (IHp1 _ _ _ H1 Heqo), p; clear IHp1.
-    destruct (IHp2 _ _ _ H2 Heqo0), p; clear IHp2.
-    exists (x ∘ x0).
-    split.
-      inversion_clear H0; cat.
+  simpl; intros.
+  destruct (term_append f2 (Identity x)); simpl in *.
+  - repeat equalities; simpl_eq.
     admit.
+  - admit.
+  - simpl.
 Admitted.
 
-Theorem denote_normalize {p dom cod} :
-  (* Term_well_typed_bool arrs dom cod p = true -> *)
-  denote dom cod p ≈ normalize_denote dom cod (normalize p).
+Lemma normalize_equiv C objs arrs x y f f' :
+  @term_denote C objs arrs x y f = Some f' ->
+  @term_denote C objs arrs x y (term_append f (Identity x)) ≈ Some f'.
 Proof.
-  destruct (denote dom cod p) eqn:?.
-    destruct (normalize_denote dom cod (normalize p)) eqn:?.
-      apply normalize_sound in Heqo0.
-        destruct Heqo0.
-        equalities.
-        red.
-        rewrite e0 in Heqo.
-        rewrite e.
-        now inversion_clear Heqo.
-      now apply denote_well_typed in Heqo.
-    admit.
-  
-  generalize dependent cod.
-  generalize dependent dom.
-  induction p as [o|a|]; intros.
-  - repeat equalities; reflexivity.
+  intros.
+  generalize dependent y.
+  generalize dependent x.
+  induction f; intros.
+  - simpl in *; repeat equalities.
+    inversion_clear H.
+    reflexivity.
   - simpl in *.
-    destruct (get_arr a); auto.
-    destruct s, s.
-    simpl_eq.
-    destruct p, p, e, e0.
-    repeat destruct (Pos.eq_dec _ _); auto.
-    destruct e, e0; cat.
-  - simpl normalize.
-    simpl denote.
-    specialize (IHp1 (TermCod arrs p2) cod).
-    specialize (IHp2 dom (TermCod arrs p2)).
-    repeat destruct (denote _ _ _); symmetry.
-Admitted.
-
-Theorem normalize_apply dom cod : ∀ f g,
-  Term_well_typed_bool arrs dom cod f = true ->
-  Term_well_typed_bool arrs dom cod g = true ->
-  ArrowList_beq (normalize f) (normalize g) = true ->
-  normalize_denote dom cod (normalize f) ||| false = true ->
-  denote dom cod f ≈ denote dom cod g.
-Proof.
-  intros.
-  apply Term_well_typed_bool_sound in H.
-  apply Term_well_typed_bool_sound in H0.
-  pose proof (ArrowList_well_typed_sound arrs H).
-  apply (ArrowList_beq_eq arrs) in H1.
-  destruct (normalize_denote dom cod (normalize f)) eqn:?; try discriminate.
-  destruct (normalize_sound H Heqo), p.
-  rewrite e0; clear e0.
-  rewrite H1 in Heqo; clear H1.
-  destruct (normalize_sound H0 Heqo), p.
-  rewrite e1; clear e1.
-  red.
-  rewrite <- e, <- e0.
-  reflexivity.
+    destruct (arrs a); [|discriminate].
+    destruct s, s; equalities.
+    equalities'; auto.
+    equalities'; auto.
+    equalities; [|discriminate].
+    inversion_clear H.
+    reflexivity.
+  - simpl in H.
+    destruct (term_denote _ _ _ _ f1) eqn:?; [|discriminate].
+    destruct (term_denote _ _ _ _ f2) eqn:?; [|discriminate].
+    inversion_clear H.
+    specialize (IHf1 _ _ _ Heqo); clear Heqo.
+    specialize (IHf2 _ _ _ Heqo0); clear Heqo0.
+    now apply term_denote_term_append.
 Qed.
 
-Corollary normalize_denote_terms dom cod : ∀ f g,
-  Term_well_typed_bool arrs dom cod f = true ->
-  Term_well_typed_bool arrs dom cod g = true ->
-  ArrowList_beq (normalize f) (normalize g) = true ->
-  normalize_denote dom cod (normalize f) ||| false = true ->
-  normalize_denote dom cod (normalize f)
-    ≈ normalize_denote dom cod (normalize g) ->
-  denote dom cod f ≈ denote dom cod g.
-Proof. intros; apply normalize_apply; auto. Qed.
-
-Corollary normalize_denote_terms_impl dom cod : ∀ f g,
-  ArrowList_beq (normalize f) (normalize g) = true ->
-  normalize_denote dom cod (normalize f)
-    ≈ normalize_denote dom cod (normalize g).
+Lemma normalize_decides C objs arrs x y f f' g g' :
+  @term_denote C objs arrs x y f = Some f' ->
+  @term_denote C objs arrs x y g = Some g' ->
+  term_beq (term_append f (Identity x)) (term_append g (Identity x)) = true ->
+  f' ≈ g'.
 Proof.
   intros.
-  apply (ArrowList_beq_eq arrs) in H.
-  now rewrite H.
-Qed.
-
-Definition expr_tauto : forall env t, [expr_denote env t].
-Proof.
-  intros; refine (Reduce (expr_backward (andImpl t) env)); auto.
-  assert (H : True \/ True \/ True \/ True \/ True) by admit.
-  inversion H; limit 0.
-Defined.
-
-Lemma expr_sound env t :
-  (if expr_tauto env t then True else False) -> expr_denote env t.
-Proof.
-  unfold expr_tauto; destruct t, (expr_backward _ env); tauto.
+  apply normalize_equiv in H.
+  apply normalize_equiv in H0.
+  pose proof (@term_denote_proper C objs arrs x y _ _ H1).
+  rewrite <- X in H0; clear X.
+  rewrite H in H0; clear H.
+  red in H0.
+  assumption.
 Qed.
 
 End Decide.
