src/Denote.v
@@ -26,23 +26,28 @@ Context {C : Category}.
 Variable objs : obj_idx -> C.
 Variable arrs : ∀ f : arr_idx, option (∃ x y, objs x ~{C}~> objs y).
 
-Fixpoint term_denote {dom cod} (e : Term dom cod) :
-  option (objs dom ~{C}~> objs cod) :=
+Fixpoint term_denote dom cod (e : Term) : option (objs dom ~{C}~> objs cod) :=
   match e with
-  | Identity _ => Some id
-  | @Morph x y a =>
+  | Identity _ =>
+      match Eq_eq_dec cod dom with
+      | left edom =>
+        Some (rew [fun x => objs x ~{ C }~> objs cod] edom in @id _ (objs cod))
+      | right _ => None
+      end
+  (* jww (2017-08-02): Why does morph need [obj_idx] arguments? *)
+  | Morph _ _ a =>
     match arrs a with
     | Some (x'; (y'; f)) =>
-      match Eq_eq_dec x' x, Eq_eq_dec y' y with
+      match Eq_eq_dec x' dom, Eq_eq_dec y' cod with
       | left edom, left ecod =>
-        Some (rew [fun x => objs x  ~{ C }~> objs y] edom in
+        Some (rew [fun x => objs x  ~{ C }~> objs cod] edom in
               rew [fun y => objs x' ~{ C }~> objs y] ecod in f)
       | _, _ => None
       end
     | _ => None
     end
-  | Compose f g =>
-    match term_denote f, term_denote g with
+  | Compose m f g =>
+    match term_denote m cod f, term_denote dom m g with
     | Some f, Some g => Some (f ∘ g)
     | _, _ => None
     end
@@ -52,7 +57,7 @@ Fixpoint expr_denote (e : Expr) : Type :=
   match e with
   | Top           => True
   | Bottom        => False
-  | Equiv _ _ f g => term_denote f ≈ term_denote g
+  | Equiv x y f g => term_denote x y f ≈ term_denote x y g
   | Not p         => expr_denote p -> False
   | And p q       => expr_denote p ∧ expr_denote q
   | Or p q        => expr_denote p + expr_denote q
@@ -71,6 +76,6 @@ Definition objs := (fun _ : obj_idx => x).
 Eval simpl in @expr_denote C objs
   (fun i => if Pos.eqb i 1 then Some (1; (1; f)) else
             if Pos.eqb i 2 then Some (1; (1; g)) else Some (1; (1; h)))%positive
-  (Equiv 1 1 (@Compose 1 1 1 (@Morph 1 1 1) (@Compose 1 1 1 (@Morph 1 1 2) (@Morph 1 1 3)))
-             (@Compose 1 1 1 (@Compose 1 1 1 (@Morph 1 1 1) (@Morph 1 1 2)) (@Morph 1 1 3)))%positive.
+  (Equiv 1 1 (@Compose 1 (@Morph 1) (@Compose 1 (@Morph 2) (@Morph 3)))
+             (@Compose 1 (@Compose 1 (@Morph 1) (@Morph 2)) (@Morph 3)))%positive.
 *)
