src/Logic.v
@@ -1,0 +1,252 @@
+Set Warnings "-notation-overridden".
+
+Require Import Coq.Program.Program.
+Require Import Coq.Bool.Bool.
+Require Import Coq.Arith.Bool_nat.
+Require Import Coq.Arith.PeanoNat.
+Require Import Coq.PArith.PArith.
+Require Import Coq.Lists.List.
+Require Import Coq.omega.Omega.
+Require Import Recdef.
+
+Require Import Category.Lib.
+Require Import Category.Theory.Functor.
+
+Require Import Solver.Lib.
+Require Import Solver.Expr.
+Require Import Solver.Denote.
+Require Import Solver.Decide.
+
+Generalizable All Variables.
+
+Section Logic.
+
+Open Scope partial_scope.
+
+Definition subst_all_expr (x : Expr) (xs : list (Expr * Expr)) : Expr := x.
+
+Lemma expr_size_subst q defs : expr_size (subst_all_expr q defs) = expr_size q.
+Proof.
+  reflexivity.
+Qed.
+
+Program Fixpoint expr_forward
+        {C : Category}
+        (objs : obj_idx -> C)
+        (arrs : ∀ f : arr_idx, option (∃ x y, objs x ~{C}~> objs y))
+        (t : Expr)
+        (hyp : Expr)
+        (cont : forall C objs' arrs' defs',
+           [@expr_denote C objs' arrs' (subst_all_expr t defs')]) :
+  [expr_denote objs arrs hyp -> expr_denote objs arrs t] :=
+  match hyp with
+  | Top           => Reduce (cont C objs arrs nil)
+  | Bottom        => Yes
+  | Equiv x y f g => No         (* jww (2017-08-02): TODO *)
+  | Not p         => No         (* jww (2017-08-02): TODO *)
+  | And p q       => No         (* jww (2017-08-02): TODO *)
+  | Or p q        => if expr_forward objs arrs t p cont
+                     then Reduce (expr_forward objs arrs t q cont)
+                     else No
+  | Impl _ _      => Reduce (cont C objs arrs nil)
+  end.
+Next Obligation. contradiction. Defined.
+Next Obligation. intuition. Defined.
+
+Program Fixpoint expr_backward
+        {C : Category}
+        (objs : obj_idx -> C)
+        (arrs : ∀ f : arr_idx, option (∃ x y, objs x ~{C}~> objs y))
+        (t : Expr)
+        {measure (expr_size t)} : [expr_denote objs arrs t] :=
+  match t with
+  | Top => Yes
+  | Bottom => No
+  | Equiv x y f g => _
+  | Not p         =>
+    match expr_backward objs arrs p with
+    | Proved _ _  => No
+    | Uncertain _ => Yes
+    end
+  | And p q       =>
+    match expr_backward objs arrs p with
+    | Proved _ _  => Reduce (expr_backward objs arrs q)
+    | Uncertain _ => No
+    end
+  | Or p q        =>
+    match expr_backward objs arrs p with
+    | Proved _ _  => Yes
+    | Uncertain _ => Reduce (expr_backward objs arrs q)
+    end
+  | Impl p q      =>
+    expr_forward objs arrs q p
+                 (fun C objs' arrs' defs' =>
+                    @expr_backward C objs' arrs' (subst_all_expr q defs') _)
+  end.
+Next Obligation.
+  destruct (term_denote objs arrs x y f) eqn:?.
+    destruct (term_denote objs arrs x y g) eqn:?.
+      destruct (term_beq (term_append f (Identity x))
+                         (term_append g (Identity x))) eqn:?.
+        apply Proved.
+        eapply normalize_decides; eauto.
+      apply Uncertain.
+    apply Uncertain.
+  apply Uncertain.
+Defined.
+Next Obligation.
+Admitted.
+Next Obligation. abstract omega. Defined.
+Next Obligation. abstract omega. Defined.
+Next Obligation. abstract omega. Defined.
+Next Obligation. abstract omega. Defined.
+Next Obligation.
+  simpl; rewrite expr_size_subst; omega.
+Defined.
+
+(*
+Theorem normalize_sound {p dom cod f} :
+  Term_well_typed arrs dom cod p ->
+  normalize_denote dom cod (normalize p) = Some f ->
+  ∃ f', f ≈ f' ∧ denote dom cod p = Some f'.
+Proof.
+  generalize dependent cod.
+  generalize dependent dom.
+  induction p as [o|a|]; simpl in *; intros; equalities.
+  - exists f; repeat equalities; reflexivity.
+  - exists f.
+    destruct (get_arr a); [|discriminate].
+    repeat equalities; reflexivity.
+  - apply normalize_compose in H0; equalities; subst.
+    + destruct (Eq_eq_dec (ArrowList_dom arrs (normalize p1))
+                          (TermCod arrs p2)).
+      * rewrite <- e in *.
+        destruct (IHp1 _ _ _ H1 a2), (IHp2 _ _ _ H2 b0).
+        equalities.
+        rewrite e3, e1.
+        eexists; intuition.
+        now rewrite <- e0, <- e2.
+      * pose proof (ArrowList_normalize_dom_cod_sound arrs H2);
+        equalities.
+        now rewrite a1 in H3.
+    + clear IHp1 IHp2.
+      pose proof (ArrowList_normalize_dom_cod_sound arrs H1).
+      pose proof (ArrowList_normalize_dom_cod_sound arrs H2).
+      equalities.
+      now rewrite H3.
+Qed.
+
+Theorem normalize_sound_r {p dom cod f} :
+  Term_well_typed arrs dom cod p ->
+  denote dom cod p = Some f ->
+  ∃ f', f ≈ f' ∧ normalize_denote dom cod (normalize p) = Some f'.
+Proof.
+  generalize dependent cod.
+  generalize dependent dom.
+  induction p as [o|a|]; simpl in *; intros; equalities.
+  - exists f; repeat equalities; reflexivity.
+  - exists f.
+    destruct (get_arr a); [|discriminate].
+    repeat equalities; reflexivity.
+  - destruct (denote (TermCod arrs p2) cod p1) eqn:?; [|discriminate].
+    destruct (denote dom (TermCod arrs p2) p2) eqn:?; [|discriminate].
+    destruct (IHp1 _ _ _ H1 Heqo), p; clear IHp1.
+    destruct (IHp2 _ _ _ H2 Heqo0), p; clear IHp2.
+    exists (x ∘ x0).
+    split.
+      inversion_clear H0; cat.
+    admit.
+Admitted.
+
+Theorem denote_normalize {p dom cod} :
+  (* Term_well_typed_bool arrs dom cod p = true -> *)
+  denote dom cod p ≈ normalize_denote dom cod (normalize p).
+Proof.
+  destruct (denote dom cod p) eqn:?.
+    destruct (normalize_denote dom cod (normalize p)) eqn:?.
+      apply normalize_sound in Heqo0.
+        destruct Heqo0.
+        equalities.
+        red.
+        rewrite e0 in Heqo.
+        rewrite e.
+        now inversion_clear Heqo.
+      now apply denote_well_typed in Heqo.
+    admit.
+  
+  generalize dependent cod.
+  generalize dependent dom.
+  induction p as [o|a|]; intros.
+  - repeat equalities; reflexivity.
+  - simpl in *.
+    destruct (get_arr a); auto.
+    destruct s, s.
+    simpl_eq.
+    destruct p, p, e, e0.
+    repeat destruct (Pos.eq_dec _ _); auto.
+    destruct e, e0; cat.
+  - simpl normalize.
+    simpl denote.
+    specialize (IHp1 (TermCod arrs p2) cod).
+    specialize (IHp2 dom (TermCod arrs p2)).
+    repeat destruct (denote _ _ _); symmetry.
+Admitted.
+
+Theorem normalize_apply dom cod : ∀ f g,
+  Term_well_typed_bool arrs dom cod f = true ->
+  Term_well_typed_bool arrs dom cod g = true ->
+  ArrowList_beq (normalize f) (normalize g) = true ->
+  normalize_denote dom cod (normalize f) ||| false = true ->
+  denote dom cod f ≈ denote dom cod g.
+Proof.
+  intros.
+  apply Term_well_typed_bool_sound in H.
+  apply Term_well_typed_bool_sound in H0.
+  pose proof (ArrowList_well_typed_sound arrs H).
+  apply (ArrowList_beq_eq arrs) in H1.
+  destruct (normalize_denote dom cod (normalize f)) eqn:?; try discriminate.
+  destruct (normalize_sound H Heqo), p.
+  rewrite e0; clear e0.
+  rewrite H1 in Heqo; clear H1.
+  destruct (normalize_sound H0 Heqo), p.
+  rewrite e1; clear e1.
+  red.
+  rewrite <- e, <- e0.
+  reflexivity.
+Qed.
+
+Corollary normalize_denote_terms dom cod : ∀ f g,
+  Term_well_typed_bool arrs dom cod f = true ->
+  Term_well_typed_bool arrs dom cod g = true ->
+  ArrowList_beq (normalize f) (normalize g) = true ->
+  normalize_denote dom cod (normalize f) ||| false = true ->
+  normalize_denote dom cod (normalize f)
+    ≈ normalize_denote dom cod (normalize g) ->
+  denote dom cod f ≈ denote dom cod g.
+Proof. intros; apply normalize_apply; auto. Qed.
+
+Corollary normalize_denote_terms_impl dom cod : ∀ f g,
+  ArrowList_beq (normalize f) (normalize g) = true ->
+  normalize_denote dom cod (normalize f)
+    ≈ normalize_denote dom cod (normalize g).
+Proof.
+  intros.
+  apply (ArrowList_beq_eq arrs) in H.
+  now rewrite H.
+Qed.
+*)
+
+Definition expr_tauto : forall C objs arrs t, [@expr_denote C objs arrs t].
+Proof.
+  intros; refine (Reduce (expr_backward objs arrs t)); auto.
+Defined.
+
+Lemma expr_sound C objs arrs t :
+  (if expr_tauto C objs arrs t then True else False) -> expr_denote objs arrs t.
+Proof.
+  unfold expr_tauto; destruct t, (expr_backward objs arrs _); tauto.
+Qed.
+
+Print Assumptions expr_tauto.
+
+End Logic.
